Compiler/Proofs/IRGeneration/ExprCore.lean
@@ -37,7 +37,8 @@ def exprBoundNames : Expr → List String
   | .externalCall _ args | .internalCall _ args | .adtConstruct _ _ args => exprListBoundNames args
   | .adtTag _ field => [field]
   | .adtField _ _ _ _ storageField => [storageField]
-  | .arrayElement name index | .arrayElementWord name index _ _ => name :: exprBoundNames index
+  | .arrayElement name index | .arrayElementWord name index _ _
+  | .arrayElementDynamicWord name index _ => name :: exprBoundNames index
   | .arrayLength name => [name]
   | .storageArrayLength name => [name]
   | .storageArrayElement name index => name :: exprBoundNames index
